\textbf{Caso \(b_1=0,b_2=0\).}
\[
\beta_{00}=\tfrac{1}{\sqrt{2}}(\ket{00}+\ket{11})
\]
\[
\xrightarrow{X^{0}\otimes I}
\tfrac{1}{\sqrt{2}}(\ket{00}+\ket{11})
\]
\[
\xrightarrow{Z^{0}\otimes I}
\tfrac{1}{\sqrt{2}}(\ket{00}+\ket{11})
\]
\[
\xrightarrow{\mathrm{CNOT}}
\tfrac{1}{\sqrt{2}}(\ket{00}+\ket{10})
\]
\[
=\bigl(\tfrac{\ket{0}+\ket{1}}{\sqrt{2}}\bigr)\otimes\ket{0}=\ket{+}\otimes\ket{0}
\]
\[
\xrightarrow{H\otimes I}
\ket{0}\otimes\ket{0}=\ket{00}
\]

\textbf{Caso \(b_1=0,b_2=1\).}
\[
\beta_{00}=\tfrac{1}{\sqrt{2}}(\ket{00}+\ket{11})
\]
\[
\xrightarrow{X^{1}\otimes I}
\tfrac{1}{\sqrt{2}}(\ket{10}+\ket{01})
\]
\[
\xrightarrow{Z^{0}\otimes I}
\tfrac{1}{\sqrt{2}}(\ket{10}+\ket{01})
\]
\[
\xrightarrow{\mathrm{CNOT}}
\tfrac{1}{\sqrt{2}}(\ket{11}+\ket{01})
\]
\[
=\bigl(\tfrac{\ket{0}+\ket{1}}{\sqrt{2}}\bigr)\otimes\ket{1}=\ket{+}\otimes\ket{1}
\]
\[
\xrightarrow{H\otimes I}
\ket{0}\otimes\ket{1}=\ket{01}
\]

\textbf{Caso \(b_1=1,b_2=0\).}
\[
\beta_{00}=\tfrac{1}{\sqrt{2}}(\ket{00}+\ket{11})
\]
\[
\xrightarrow{X^{0}\otimes I}
\tfrac{1}{\sqrt{2}}(\ket{00}+\ket{11})
\]
\[
\xrightarrow{Z^{1}\otimes I}
\tfrac{1}{\sqrt{2}}(\ket{00}-\ket{11})
\]
\[
\xrightarrow{\mathrm{CNOT}}
\tfrac{1}{\sqrt{2}}(\ket{00}-\ket{10})
\]
\[
=\bigl(\tfrac{\ket{0}-\ket{1}}{\sqrt{2}}\bigr)\otimes\ket{0}=\ket{-}\otimes\ket{0}
\]
\[
\xrightarrow{H\otimes I}
\ket{1}\otimes\ket{0}=\ket{10}
\]

\textbf{Caso \(b_1=1,b_2=1\).}
\[
\beta_{00}=\tfrac{1}{\sqrt{2}}(\ket{00}+\ket{11})
\]
\[
\xrightarrow{X^{1}\otimes I}
\tfrac{1}{\sqrt{2}}(\ket{10}+\ket{01})
\]
\[
\xrightarrow{Z^{1}\otimes I}
\tfrac{1}{\sqrt{2}}(-\ket{10}+\ket{01})
\]
\[
\xrightarrow{\mathrm{CNOT}}
\tfrac{1}{\sqrt{2}}(-\ket{11}+\ket{01})
\]
\[
=\bigl(\tfrac{\ket{0}-\ket{1}}{\sqrt{2}}\bigr)\otimes\ket{1}=\ket{-}\otimes\ket{1}
\]
\[
\xrightarrow{H\otimes I}
\ket{1}\otimes\ket{1}=\ket{11}
\]
